Start etcdserver proof; verify most of `idutil`, but need to add `w16` to
finish it.

new/proof/go_etcd_io/etcd/server/v3/etcdserver.v
@@ -1,7 +1,7 @@
 Require Export New.code.go_etcd_io.etcd.server.v3.etcdserver.
 Require Export New.generatedproof.go_etcd_io.etcd.server.v3.etcdserver.
 Require Export New.proof.proof_prelude.
-From New.proof Require Import context log fmt.
+From New.proof Require Import context log fmt go_etcd_io.etcd.pkg.v3.idutil.
 
 Section wps.
 Context `{hG: heapGS Σ, !ffi_semantics _ _}.
@@ -13,8 +13,6 @@ Context `{!globalsGS Σ} {go_ctx : GoContext}.
 #[global] Instance : IsPkgInit apply.apply := define_is_pkg_init True%I.
 #[global] Instance : IsPkgInit v3.auth.auth := define_is_pkg_init True%I.
 #[global] Instance : IsPkgInit wait := define_is_pkg_init True%I.
-#[global] Instance : IsPkgInit math := define_is_pkg_init True%I.
-#[global] Instance : IsPkgInit idutil := define_is_pkg_init True%I.
 #[global] Instance : IsPkgInit prometheus := define_is_pkg_init True%I.
 #[global] Instance : IsPkgInit errors.errors := define_is_pkg_init True%I.
 #[global] Instance : IsPkgInit config := define_is_pkg_init True%I.
@@ -31,12 +29,47 @@ Proof.
   (* Need to translate traceutil.StartTimeKey. so struct literal can be allocated *)
 Abort.
 
-Lemma wp_EtcdServer__processInternalRaftRequestOnce (s : loc) (ctx : context.Context.t) (r : loc) :
-  {{{ is_pkg_init etcdserver }}}
+Axiom EtcdServer_names : Type.
+Implicit Type γ : EtcdServer_names.
+
+Definition is_EtcdServer (s : loc) γ : iProp Σ :=
+  ∃ (reqIDGen : loc),
+    "reqIDGen" ∷ s ↦s[etcdserver.EtcdServer :: "reqIDGen"]□ reqIDGen ∗
+    "_" ∷ True
+.
+#[global] Opaque is_EtcdServer.
+#[local] Transparent is_EtcdServer.
+Instance : ∀ s γ, Persistent (is_EtcdServer s γ).
+Proof. apply _. Qed.
+
+Axiom wp_EtcdServer__getAppliedIndex : ∀ s γ,
+  {{{ is_pkg_init etcdserver ∗ is_EtcdServer s γ }}}
+    s @ (ptrT.id etcdserver.EtcdServer.id) @ "getAppliedIndex" #()
+  {{{ (a : w64), RET #a; True }}}.
+
+Axiom wp_EtcdServer__getCommittedIndex : ∀ s γ,
+  {{{ is_pkg_init etcdserver ∗ is_EtcdServer s γ }}}
+    s @ (ptrT.id etcdserver.EtcdServer.id) @ "getCommittedIndex" #()
+  {{{ (a : w64), RET #a; True }}}.
+
+Lemma wp_EtcdServer__processInternalRaftRequestOnce (s : loc) γ (ctx : context.Context.t) (r : loc) :
+  {{{ is_pkg_init etcdserver ∗ is_EtcdServer s γ }}}
     s @ (ptrT.id etcdserver.EtcdServer.id) @ "processInternalRaftRequestOnce" #ctx #r
   {{{ RET #(); True }}}.
 Proof.
-  wp_start.
-Abort.
+  wp_start as "#Hsrv".
+  wp_apply wp_with_defer as "%defer Hdefer" . simpl subst.
+  wp_auto. wp_apply (wp_EtcdServer__getAppliedIndex with "[$Hsrv]") as "%ai _".
+  wp_apply (wp_EtcdServer__getCommittedIndex with "[$Hsrv]") as "%ci _".
+  wp_if_destruct.
+  {
+    (* FIXME: declare then access init predicate of errors. *)
+    admit.
+  }
+  wp_auto.
+  iNamed "Hsrv".
+  wp_auto.
+  (* FIXME: verify [idutil] library. *)
+Admitted.
 
 End wps.
