new/proof/go_etcd_io/etcd/pkg/v3/idutil.v
@@ -1,0 +1,56 @@
+Require Export New.generatedproof.go_etcd_io.etcd.pkg.v3.idutil.
+Require Export New.proof.proof_prelude.
+From New.proof Require Import time math sync.atomic.
+
+Section wps.
+Context `{hG: heapGS Σ, !ffi_semantics _ _}.
+Context `{!globalsGS Σ} {go_ctx : GoContext}.
+
+#[global] Instance : IsPkgInit math := define_is_pkg_init True%I.
+#[global] Instance : IsPkgInit idutil := define_is_pkg_init True%I.
+
+Definition is_Generator (g : loc) : iProp Σ :=
+  ∃ (prefix : w64),
+    "#prefix" ∷ g ↦s[idutil.Generator :: "prefix"]□ prefix ∗
+    "#suffix" ∷ inv nroot (∃ (suffix : w64),
+          struct.field_ref_f idutil.Generator "suffix" g ↦ suffix
+      ) ∗
+    "_" ∷ True.
+#[global] Opaque is_Generator.
+#[local] Transparent is_Generator.
+Instance : ∀ s, Persistent (is_Generator s).
+Proof. apply _. Qed.
+
+Lemma wp_lowbit (x n : w64) :
+  {{{ is_pkg_init idutil }}}
+    @! idutil.lowbit #x #n
+  {{{ (y : w64), RET #y; True }}}.
+Proof.
+  wp_start. wp_auto. iApply "HΦ". done.
+Qed.
+
+Lemma wp_Generator__Next g :
+  {{{ is_pkg_init idutil ∗ is_Generator g }}}
+    g @ (ptrT.id idutil.Generator.id) @ "Next" #()
+  {{{ (i : w64), RET #i; True }}}.
+Proof.
+  wp_start as "H". iNamedSuffix "H" "_g".
+  wp_auto. wp_bind.
+  wp_apply wp_AddUint64.
+  iInv "suffix_g" as ">Hi" "Hclose".
+  iApply fupd_mask_intro. { solve_ndisj. } iIntros "Hmask".
+  iNamed "Hi". iFrame. iIntros "Hi".
+  iMod "Hmask". iMod ("Hclose" with "[$Hi]") as "_". iModIntro.
+  wp_auto. wp_apply wp_lowbit as "%y _". iApply "HΦ". done.
+Qed.
+
+(* FIXME: need w16  *)
+(*
+Lemma wp_NewGenerator (memberID : w16) (now : time.Time.t) :
+  {{{ is_pkg_init idutil }}}
+    @! idutil.NewGenerator #memberID #now
+  {{{ RET #(); True }}}.
+Proof.
+Qed. *)
+
+End wps.
