new/proof/time.v
@@ -1,0 +1,11 @@
+Require Export New.generatedproof.time.
+
+Section defns.
+Context `{hG: heapGS Σ, !ffi_semantics _ _}.
+Context `{!globalsGS Σ} {go_ctx : GoContext}.
+Context `{contextG Σ}.
+
+#[global] Instance : IsPkgInit time := define_is_pkg_init True%I.
+#[global] Instance : GetIsPkgInitWf time := build_get_is_pkg_init_wf.
+
+End defns.
